meeting
git-svn-id: orca@478

C-verifier/src/Midend-IVL/Isabelle-UTP-Extended/examples/TotalCorrectness/Rel/examples_vcg_Floyd.thy
@@ -318,9 +318,9 @@ lemma f_rule:
   unfolding f_def using assms INDEP
   by rel_simp
 
-definition "EXINV l P \<equiv> \<^bold>\<exists>st \<bullet> P\<lbrakk>(\<guillemotleft>st\<guillemotright> \<oplus> &\<Sigma> on &l)/&\<Sigma>\<rbrakk>" (* P holds on st[&l/l]     *)    
+definition (in -) "EXINV l P \<equiv> \<^bold>\<exists>st \<bullet> P\<lbrakk>(\<guillemotleft>st\<guillemotright> \<oplus> &\<Sigma> on &l)/&\<Sigma>\<rbrakk>" (* P holds on st[&l/l]     *)    
 
-lemma
+lemma antiframe_rule[hoare_rules]:
   assumes "vwb_lens a"  "\<lbrace>P\<rbrace> c \<lbrace>Q\<rbrace>\<^sub>u"
   shows "\<lbrace>P\<rbrace> a:[c] \<lbrace> (\<exists>a \<bullet> P) \<and> (EXINV a Q) \<rbrace>\<^sub>u"  
   using assms unfolding EXINV_def
@@ -330,13 +330,117 @@ lemma
     
     
     
+    
+    
+declare assigns_floyd_r[hoare_rules del]    
+lemma (in -) assigns_floyd_rX [hoare_rules]:
+  assumes \<open>vwb_lens x\<close>
+  shows   \<open>\<lbrace>p\<rbrace>x :== e\<lbrace>(\<exists>x \<bullet> p) \<and> (\<^bold>\<exists>v \<bullet> &x =\<^sub>u e\<lbrakk>\<guillemotleft>v\<guillemotright>/x\<rbrakk>)  \<rbrace>\<^sub>u\<close>
+  apply (insert assms)
+  apply pred_simp
+  apply transfer
+  apply (rule)  
+  apply (rule_tac x = \<open>get\<^bsub>x\<^esub> a\<close> in exI)
+  (*subgoal for a x p e
+   apply (rule exI[where x="get\<^bsub>x\<^esub> a"])*)
+  apply auto
+  apply (rule_tac x = \<open>get\<^bsub>x\<^esub> a\<close> in exI)
+  apply auto
+  done
+    
+lemma (in -) modified_assign_rule:
+  assumes \<open>vwb_lens x\<close>
+  shows   \<open>\<lbrace>p\<rbrace>x :== e\<lbrace>(\<exists>x \<bullet> p) \<rbrace>\<^sub>u\<close>
+  apply (rule hoare_post_weak)
+  apply (rule assigns_floyd_rX)  
+  apply fact
+  apply pred_simp
+  done  
+    
+lemma (in -) EXINV_pull_out_sublens:
+  fixes x l
+  assumes A: "vwb_lens x" "vwb_lens l"
+  defines "XX\<equiv>x;\<^sub>Ll"
+  shows "EXINV l (\<exists>XX \<bullet> P ) = (\<exists>XX \<bullet> EXINV l P)"
+  unfolding EXINV_def XX_def using A 
+  by pred_blast
+    
+lemma (in -) EXINV_drop_indep:
+  fixes x l
+  assumes A: "vwb_lens l1" "vwb_lens l2" "l1\<bowtie>l2"
+  shows "EXINV l1 (\<exists>l2 \<bullet> P ) = (EXINV l1 P)"
+  unfolding EXINV_def using A 
+  apply pred_simp
+  by (metis lens_indep_def vwb_lens_wb wb_lens.get_put)  
+    
+lemma (in -) lens_indep_right_ext' [intro, simp]:
+  "z \<bowtie> x \<Longrightarrow> x \<bowtie> (y ;\<^sub>L z)"
+  using lens_indep_sym by blast  
+  
+lemma (in -) lens_indep_left_ext' [intro, simp]:
+  "x \<bowtie> z \<Longrightarrow> (y ;\<^sub>L z) \<bowtie> x"
+  using lens_indep_sym by blast  
+    
+(*lemmas [simp] = lens_indep_right_ext lens_indep_left_ext*)
+    
+    
+lemma conj_ex2_move_front: "l \<sharp> P \<Longrightarrow> (P \<and> (\<exists>l \<bullet> Q)) = (\<exists>l \<bullet> P \<and> Q )"
+  by pred_simp
+    
+lemma (in -) dep_unrest_ex:
+  fixes x l
+  assumes A: "vwb_lens x" "vwb_lens l"
+  defines "XX \<equiv> x;\<^sub>Ll"
+  shows "XX \<sharp> (\<exists> l \<bullet> F)"
+  unfolding XX_def using A
+  by pred_simp  
+    
+lemma (in -) 
+  assumes "vwb_lens l"
+  shows "((\<exists> l \<bullet> F) \<and> EXINV l F) = F"
+  using assms
+  unfolding EXINV_def  
+  apply pred_simp
+  apply transfer  
+    oops
+      
+lemma (in -) "(\<exists>x. P x st) \<and> (\<exists>x. Q x st) \<Longrightarrow> \<exists>x. P x st \<and> Q x st" oops   
+  
+    
+    
+    
 lemma 
   assumes "vwb_lens r"
   shows "\<lbrace> F \<rbrace> f r a \<lbrace> \<exists> r \<bullet> \<exists> Gret \<bullet> F \<rbrace>\<^sub>u"
-  unfolding f_def using INDEP assms apply -
-  apply (exp_vcg)  
-  apply rel_simp
-  
+  unfolding f_def using INDEP assms
+  (*supply assigns_floyd_rX [hoare_rules del]  
+  supply modified_assign_rule[hoare_rules]  *)
+  apply -  
+  apply (exp_vcg)
+  apply (simp add: EXINV_pull_out_sublens EXINV_drop_indep conj_ex2_move_front dep_unrest_ex)
+  unfolding EXINV_def  
+  apply pred_simp  
+    
+  apply (subst conj_ex2_move_front)  
+    
+    
+    
+oops    
+  apply (subst EXINV_drop_indep)  
+  apply simp  
+  apply simp  
+  apply (rule lens_indep_sym)
+  solve_direct  
+    
+  using lens_indep_sym apply blast  
+  apply simp  
+    
+oops    
+  apply (solve_vcg)  
+  apply pred_simp
+    
+    
+  apply (simp add: vwb_lens_wb[THEN wb_lens.get_put])
   
     
 lemma "\<lbrace> &Ly=\<^sub>u\<guillemotleft>val2\<guillemotright> \<and> &Lx=\<^sub>u\<guillemotleft>val\<guillemotright> \<rbrace> f Lx (&Lx) \<lbrace> &Ly=\<^sub>u\<guillemotleft>val2\<guillemotright> \<and> &Lx=\<^sub>u\<guillemotleft>val+1\<guillemotright> \<rbrace>\<^sub>u"
